PsBool.v
@@ -2,12 +2,12 @@ Require Import Basics Relations List.
 Require Import Utils PsCore.
 
 Definition instfalse_spec (i1 : inst) : Prop :=
-  forall (i2 i3 : inst) (vs ps : stack),
-    (i3 :: i2 :: vs, i1 :: ps) |=>* (i3 :: i2 :: vs, ps).
+  forall (i2 i3 : inst) (vs cs : stack),
+    (i3 :: i2 :: vs, i1 :: cs) |=>* (i3 :: i2 :: vs, cs).
 
 Definition insttrue_spec (i1 : inst) : Prop :=
-  forall (i2 i3 : inst) (vs ps : stack),
-    (i3 :: i2 :: vs, i1 :: ps) |=>* (i2 :: i3 :: vs, ps).
+  forall (i2 i3 : inst) (vs cs : stack),
+    (i3 :: i2 :: vs, i1 :: cs) |=>* (i2 :: i3 :: vs, cs).
 
 Definition instbool_spec (b : bool) (i : inst) : Prop :=
   if b then insttrue_spec i else instfalse_spec i.
@@ -27,9 +27,9 @@ Qed.
 Definition instnot := instseq [ instpush ; instswap ; instcons ].
 
 Lemma instnot_proof :
-  forall (b : bool) (i1 : inst) (vs ps : stack), instbool_spec b i1 ->
+  forall (b : bool) (i1 : inst) (vs cs : stack), instbool_spec b i1 ->
     exists i2 : inst, instbool_spec (negb b) i2 /\
-    (i1 :: vs, instnot :: ps) |=>* (i2 :: vs, ps).
+    (i1 :: vs, instnot :: cs) |=>* (i2 :: vs, cs).
   intros ; evalauto ; destruct b ;
     repeat intro ; evalauto ; evalpartial H ; evalauto.
 Qed.
@@ -43,28 +43,28 @@ Definition instif := instseq
     instexec ;
     instexec ; instswap ; instpop ].
 
-Lemma eval_instif : forall (b : bool) (i1 i2 i3 : inst) (vs ps : stack),
-  instbool_spec b i1 -> (i3 :: i2 :: i1 :: vs, instif :: ps) |=>*
-    ((if b then i2 else i3) :: vs, ps).
+Lemma eval_instif : forall (b : bool) (i1 i2 i3 : inst) (vs cs : stack),
+  instbool_spec b i1 -> (i3 :: i2 :: i1 :: vs, instif :: cs) |=>*
+    ((if b then i2 else i3) :: vs, cs).
   intros.
   destruct b ; evalauto ; evalpartial H ; evalauto.
 Qed.
 
 Definition instexecif := instseq [ instif ; instexec ].
 
-Lemma eval_instexecif : forall (b : bool) (i1 i2 i3 : inst) (vs ps : stack),
-  instbool_spec b i1 -> (i3 :: i2 :: i1 :: vs, instexecif :: ps) |=>*
-    (vs, (if b then i2 else i3) :: ps).
+Lemma eval_instexecif : forall (b : bool) (i1 i2 i3 : inst) (vs cs : stack),
+  instbool_spec b i1 -> (i3 :: i2 :: i1 :: vs, instexecif :: cs) |=>*
+    (vs, (if b then i2 else i3) :: cs).
   intros.
   destruct b ; evalauto ; evalpartial H ; evalauto.
 Qed.
 
 Definition instxor := instcons.
 
-Lemma instxor_proof : forall (b1 b2 : bool) (i1 i2 : inst) (vs ps : stack),
+Lemma instxor_proof : forall (b1 b2 : bool) (i1 i2 : inst) (vs cs : stack),
   instbool_spec b1 i1 -> instbool_spec b2 i2 ->
     exists i3 : inst, instbool_spec (xorb b1 b2) i3 /\
-    (i2 :: i1 :: vs, instxor :: ps) |=>* (i3 :: vs, ps).
+    (i2 :: i1 :: vs, instxor :: cs) |=>* (i3 :: vs, cs).
   intros ; evalauto ; destruct b1, b2 ; repeat intro ;
     evalauto ; evalpartial H ; evalpartial H0 ; evalauto.
 Qed.
